ConcreteF.eca : completed Handle.eca    : TODO

sha3/proof/smart_counter/SLCommon.ec
@@ -39,16 +39,34 @@ clone import RndO.GenEager as F with
   op sampleto <- fun (_:block list)=> bdistr
   proof * by exact Block.DBlock.dunifin_ll.
 
+
+module Redo = {
+  var prefixes : (block list, state) fmap
+
+  proc init() : unit = {
+    prefixes <- map0.[[] <- (b0,c0)];
+  }
+}.
+
 (** We can now define the squeezeless sponge construction **)
 module SqueezelessSponge (P:DPRIMITIVE): FUNCTIONALITY = {
-  proc init () = {} 
+  proc init () = {
+    Redo.init();
+  } 
 
   proc f(p : block list): block = {
     var (sa,sc) <- (b0,c0);
+    var i : int <- 0;
 
-    while (p <> []) { (* Absorption *)
-      (sa,sc) <@ P.f((sa +^ head witness p,sc));
-      p <- behead p;
+    while (i < size p) { (* Absorption *)
+      if (take (i+1) p \in dom Redo.prefixes) {
+        (sa,sc) <- oget Redo.prefixes.[take (i+1) p];
+      } else {
+        (sa,sc) <- (sa +^ nth witness p i, sc);
+        (sa,sc) <@ P.f((sa,sc));
+        Redo.prefixes.[take (i+1) p] <- (sa,sc);
+      }
+      i <- i + 1;
     }
 
     return sa;          (* Squeezing phase (non-iterated) *)
@@ -199,6 +217,32 @@ move=>e2 l2 Hind1 e1 l1 Hind2=>//=.
 by case(e1=e2)=>[->//=/#|//=].
 qed.
 
+lemma take_take (l : 'a list) (i j : int) :
+    take i (take j l) = take (min i j) l.
+proof.
+case(i <= j)=>Hij.
++ case(j < size l)=>Hjsize;last smt(take_oversize).
+  case(0 <= i)=>Hi0;last smt(take_le0).
+  apply (eq_from_nth witness);1:smt(size_take).
+  move=>k;rewrite !size_take//=1:/# Hjsize/=.
+  cut->: (if i < j then i else j) = i by rewrite/#.
+  move=>[Hk0 Hki].
+  by rewrite !nth_take//=/#.
+case(0<j)=>//=Hj0;last smt(take_le0).
+rewrite min_ler 1:/#. 
+pose l':=take j l. 
+rewrite take_oversize//=.
+rewrite/l' size_take /#.
+qed.
+
+lemma prefixe_take_leq (l1 l2 : 'a list) (i : int) :
+    i <= prefixe l1 l2 => take i l1 = take i l2.
+proof.
+move=>Hi.
+cut->:i = min i (prefixe l1 l2) by smt(min_lel).
+by rewrite-(take_take l1 i _)-(take_take l2 i _) prefixe_take.
+qed.
+
 lemma prefixe_nth (l1 l2 : 'a list) :
     let i = prefixe l1 l2 in
     forall j, 0 <= j < i => 
@@ -222,6 +266,414 @@ op get_max_prefixe (l : 'a list) (ll : 'a list list) =
   with ll = "[]" => []
   with ll = (::) l' ll' => max_prefixe l l' ll'.
 
+
+pred prefixe_inv (queries : (block list, block) fmap)
+               (prefixes : (block list, state) fmap) =
+  (forall (bs : block list),
+    bs \in dom queries => oget queries.[bs] = (oget prefixes.[bs]).`1) &&
+  (forall (bs : block list),
+    bs \in dom queries => forall i, take i bs \in dom prefixes) &&
+  (forall (bs : block list),
+    forall i, take i bs <> [] =>
+    take i bs \in dom prefixes =>
+    exists l2, (take i bs) ++ l2 \in dom queries).
+
+pred all_prefixes (prefixes : (block list, state) fmap) =
+    forall (bs : block list), bs \in dom prefixes => forall i, take i bs \in dom prefixes.
+
+lemma aux_mem_get_max_prefixe (l1 l2 : 'a list) ll :
+    max_prefixe l1 l2 ll = l2 \/ max_prefixe l1 l2 ll \in ll.
+proof.
+move:l1 l2;elim:ll=>//=l3 ll Hind l1 l2. 
+case(prefixe l1 l2 < prefixe l1 l3)=>//=hmax.
++ cut/#:=Hind l1 l3.
+cut/#:=Hind l1 l2.
+qed.
+
+
+lemma mem_get_max_prefixe (l : 'a list) ll :
+    ll <> [] => get_max_prefixe l ll  \in ll.
+proof.
+move:l;elim:ll=>//=l2 ll Hind l1. 
+exact aux_mem_get_max_prefixe.
+qed.
+
+
+lemma take_get_max_prefixe l prefixes :
+    (exists b, b  \in dom prefixes) =>
+    all_prefixes prefixes =>
+    take (prefixe l (get_max_prefixe l (elems (dom prefixes)))) l \in dom prefixes.
+proof.
+move=>nil_in_dom all_pref.
+rewrite prefixe_take all_pref memE mem_get_max_prefixe;smt(memE).
+qed.
+    
+lemma take_get_max_prefixe2 l prefixes i :
+    (exists b, b \in dom prefixes) =>
+    all_prefixes prefixes =>
+    i <= prefixe l (get_max_prefixe l (elems (dom prefixes))) =>
+    take i l \in dom prefixes.
+proof.
+move=>nil_in_dom all_pref hi. 
+rewrite (prefixe_take_leq _ _ i hi) all_pref memE mem_get_max_prefixe;smt(memE).
+qed.
+
+
+lemma prefixe_cat (l l1 l2 : 'a list) :
+    prefixe (l ++ l1) (l ++ l2) = size l + prefixe l1 l2.
+proof.
+move:l1 l2;elim l=>//=/#.
+qed.
+
+
+lemma prefixe_leq_take (l1 l2 : 'a list) i :
+    0 <= i <= min (size l1) (size l2) => 
+    take i l1 = take i l2 =>
+    i <= prefixe l1 l2.
+proof.
+move=> [hi0 himax] htake.
+rewrite-(cat_take_drop i l1)-(cat_take_drop i l2)htake. 
+rewrite prefixe_cat size_take//=;smt(prefixe_ge0).
+qed.
+
+lemma prefixe0 (l1 l2 : 'a list) :
+    prefixe l1 l2 = 0 <=> l1 = [] \/ l2 = [] \/ head witness l1 <> head witness l2 .
+proof.
+move:l2;elim:l1=>//=;1:rewrite/#;move=>e1 l1 Hind l2;move:e1 l1 Hind;elim:l2=>//=e2 l2 Hind2 e1 l1 Hind1.
+smt(prefixe_ge0).
+qed.
+
+lemma head_nth0 (l : 'a list) : head witness l = nth witness l 0.
+proof. by elim:l. qed.
+
+
+lemma get_prefixe (l1 l2 : 'a list) i :
+    0 <= i <= min (size l1) (size l2)=>
+    (drop i l1 = [] \/ drop i l2 = [] \/
+    (i < min (size l1) (size l2) /\
+    nth witness l1 i <> nth witness l2 i)) =>
+    take i l1 = take i l2 =>
+    i = prefixe l1 l2.
+proof.
+move=>[hi0 hisize] [|[]]. 
++ move=>hi. 
+  cut:=size_eq0 (drop i l1);rewrite {2}hi/=size_drop// =>h.
+  cut hsize: size l1 = i by rewrite/#. 
+  rewrite -hsize take_size.
+  rewrite-{2}(cat_take_drop (size l1) l2)=><-.
+  by rewrite-{2}(cats0 l1)prefixe_cat/#. 
++ move=>hi. 
+  cut:=size_eq0 (drop i l2);rewrite {2}hi/=size_drop// =>h.
+  cut hsize: size l2 = i by rewrite/#. 
+  rewrite -hsize take_size.
+  rewrite-{2}(cat_take_drop (size l2) l1)=>->.
+  by rewrite-{4}(cats0 l2)prefixe_cat/#. 
+move=>[himax  hnth] htake.
+rewrite-(cat_take_drop i l1)-(cat_take_drop i l2)htake. 
+rewrite prefixe_cat size_take//=.
++ cut[_ ->]:=prefixe0 (drop i l1) (drop i l2).
+  case(i = size l1)=>hi1//=.
+  + by rewrite hi1 drop_size//=.
+  case(i = size l2)=>hi2//=.
+  + by rewrite hi2 drop_size//=.
+  by rewrite 2!head_nth0 nth_drop//=nth_drop//= hnth.
+rewrite/#.
+qed.
+
+lemma get_max_prefixe_leq (l1 l2 : 'a list) (ll : 'a list list) :
+    prefixe l1 l2 <= prefixe l1 (max_prefixe l1 l2 ll).
+proof.
+move:l1 l2;elim:ll=>//=/#.
+qed.
+
+lemma get_max_prefixe_is_max (l1 l2 : 'a list) (ll : 'a list list) :
+    forall l3, l3 \in ll => prefixe l1 l3 <= prefixe l1 (max_prefixe l1 l2 ll).
+proof.
+move:l1 l2;elim:ll=>//=. 
+move=>l4 ll Hind l1 l2 l3.
+case(prefixe l1 l2 < prefixe l1 l4)=>//=h [];smt( get_max_prefixe_leq ).
+qed.
+
+lemma get_max_prefixe_max (l : 'a list) (ll : 'a list list) :
+    forall l2, l2 \in ll => prefixe l l2 <= prefixe l (get_max_prefixe l ll).
+proof. smt(get_max_prefixe_is_max get_max_prefixe_leq). qed.
+
+lemma all_take_in (l : block list) i prefixes :
+    0 <= i <= size l =>
+    all_prefixes prefixes =>
+    take i l \in dom prefixes =>
+    i <= prefixe l (get_max_prefixe l (elems (dom prefixes))).
+proof.
+move=>[hi0 hisize] all_prefixe take_in_dom.
+cut->:i = prefixe l (take i l);2:smt(get_max_prefixe_max memE).
+apply get_prefixe. 
++ smt(size_take). 
++ by right;left;apply size_eq0;rewrite size_drop//size_take//=/#.
+smt(take_take).
+qed.
+
+lemma prefixe_inv_leq (l : block list) i prefixes queries :
+    0 <= i <= size l =>
+    elems (dom queries) <> [] =>
+    all_prefixes prefixes =>
+    take i l \in dom prefixes =>
+    prefixe_inv queries prefixes =>
+    i <= prefixe l (get_max_prefixe l (elems (dom queries))).
+proof.
+move=>h_i h_nil h_all_prefixes take_in_dom [?[h_prefixe_inv h_exist]].
+case(take i l = [])=>//=h_take_neq_nil.
++ smt(prefixe_ge0 size_eq0).
+cut[l2 h_l2_mem]:=h_exist l i h_take_neq_nil take_in_dom.
+rewrite memE in h_l2_mem.
+rewrite(StdOrder.IntOrder.ler_trans _ _ _ _ (get_max_prefixe_max _ _ _ h_l2_mem)).
+rewrite-{1}(cat_take_drop i l)prefixe_cat size_take 1:/#;smt(prefixe_ge0).
+qed.
+
+
+lemma max_prefixe_eq (l : 'a list) (ll : 'a list list) :
+    max_prefixe l l ll = l.
+proof. 
+move:l;elim:ll=>//=l2 ll Hind l1;smt( prefixe_eq prefixe_sizel).
+qed.
+
+lemma prefixe_max_prefixe_eq_size (l1 l2 : 'a list) (ll : 'a list list) :
+    l1 = l2 \/ l1 \in ll =>
+    prefixe l1 (max_prefixe l1 l2 ll) = size l1.
+proof.
+move:l1 l2;elim:ll=>//=;1:smt(prefixe_eq). 
+move=>l3 ll Hind l1 l2[->|[->|h1]].
++ rewrite prefixe_eq max_prefixe_eq;smt(max_prefixe_eq prefixe_eq prefixe_sizer).
++ rewrite prefixe_eq max_prefixe_eq. 
+  case(prefixe l3 l2 < size l3)=>//=h;1:by rewrite prefixe_eq.
+  cut h1:prefixe l3 l2 = size l3 by smt(prefixe_sizel).
+  cut: size l3 <= prefixe l3 (max_prefixe l3 l2 ll);2:smt(prefixe_sizel).
+  rewrite-h1.
+  by clear Hind l1 h h1;move:l2 l3;elim:ll=>//=l3 ll Hind l1 l2/#.
+by case(prefixe l1 l2 < prefixe l1 l3)=>//=/#.
+qed.
+
+lemma prefixe_get_max_prefixe_eq_size (l : 'a list) (ll : 'a list list) :
+    l \in ll =>
+    prefixe l (get_max_prefixe l ll) = size l.
+proof.
+move:l;elim:ll=>//;smt(prefixe_max_prefixe_eq_size).
+qed.
+
+lemma get_max_prefixe_exists (l : 'a list) (ll : 'a list list) :
+    ll <> [] =>
+    exists l2, take (prefixe l (get_max_prefixe l ll)) l ++ l2 \in ll.
+proof.
+move:l;elim:ll=>//=l2 ll Hind l1;clear Hind;move:l1 l2;elim:ll=>//=.
++ smt(cat_take_drop prefixe_take).
+move=>l3 ll Hind l1 l2.
+case( prefixe l1 l2 < prefixe l1 l3 )=>//=h/#.
+qed.
+
+lemma prefixe_geq (l1 l2 : 'a list) :
+    prefixe l1 l2 = prefixe (take (prefixe l1 l2) l1) (take (prefixe l1 l2) l2).
+proof.
+move:l2;elim:l1=>//=[/#|]e1 l1 Hind l2;elim:l2=>//=e2 l2 Hind2.
+case(e1=e2)=>//=h12.
+cut->/=:! 1 + prefixe l1 l2 <= 0 by smt(prefixe_ge0).
+rewrite h12/=/#.
+qed.
+
+lemma prefixe_take_prefixe (l1 l2 : 'a list) :
+    prefixe (take (prefixe l1 l2) l1) l2 = prefixe l1 l2.
+proof.
+move:l2;elim:l1=>//=e1 l1 Hind l2;elim:l2=>//=e2 l2 Hind2.
+case(e1=e2)=>//=h12.
+cut->/=:! 1 + prefixe l1 l2 <= 0 by smt(prefixe_ge0).
+rewrite h12/=/#.
+qed.
+
+lemma prefixe_leq_prefixe_cat (l1 l2 l3 : 'a list) :
+    prefixe l1 l2 <= prefixe (l1 ++ l3) l2.
+proof.
+move:l2 l3;elim l1=>//=;1:smt(take_le0 prefixe_ge0).
+move=>e1 l1 hind1 l2;elim:l2=>//=e2 l2 hind2 l3/#.
+qed.
+
+lemma prefixe_take_leq_prefixe (l1 l2 : 'a list) i :
+    prefixe (take i l1) l2 <= prefixe l1 l2.
+proof.
+rewrite-{2}(cat_take_drop i l1).
+move:(take i l1)(drop i l1);clear i l1=>l1 l3. 
+exact prefixe_leq_prefixe_cat.
+qed.
+
+lemma prefixe_take_geq_prefixe (l1 l2 : 'a list) i :
+    prefixe l1 l2 <= i =>
+    prefixe l1 l2 = prefixe (take i l1) l2.
+proof.
+move=>hi.
+cut:prefixe (take i l1) l2 <= prefixe l1 l2.
++ rewrite-{2}(cat_take_drop i l1) prefixe_leq_prefixe_cat.
+cut/#:prefixe l1 l2 <= prefixe (take i l1) l2.
+rewrite -prefixe_take_prefixe.
+rewrite-(cat_take_drop (prefixe l1 l2) (take i l1))take_take min_lel// prefixe_leq_prefixe_cat. 
+qed.
+
+lemma get_max_prefixe_take (l : 'a list) (ll : 'a list list) i :
+    prefixe l (get_max_prefixe l ll) <= i =>
+    get_max_prefixe l ll = get_max_prefixe (take i l) ll.
+proof.
+move:l;elim:ll=>//=l2 ll Hind l1;clear Hind;move:l1 l2;elim:ll=>//=l3 ll Hind l1 l2.
+case( prefixe l1 l2 < prefixe l1 l3 )=>//=h hi.
++ rewrite -prefixe_take_geq_prefixe//=;1:smt(get_max_prefixe_leq).
+  rewrite -prefixe_take_geq_prefixe//=;1:smt(get_max_prefixe_leq). 
+  rewrite h/=/#.
+rewrite -prefixe_take_geq_prefixe//=;1:smt(get_max_prefixe_leq).
+rewrite -prefixe_take_geq_prefixe//=;1:smt(get_max_prefixe_leq). 
+rewrite h/=/#.
+qed.
+
+
+lemma drop_prefixe_neq (l1 l2 : 'a list) :
+    drop (prefixe l1 l2) l1 = [] \/ drop (prefixe l1 l2) l1 <> drop (prefixe l1 l2) l2.
+proof.
+move:l2;elim:l1=>//=e1 l1 hind1 l2;elim:l2=>//=e2 l2 hind2/#.
+qed.
+
+
+lemma prefixe_prefixe_prefixe (l1 l2 l3 : 'a list) (ll : 'a list list) :
+    prefixe l1 l2 <= prefixe l1 l3 =>
+    prefixe l1 (max_prefixe l1 l2 ll) <= prefixe l1 (max_prefixe l1 l3 ll).
+proof.
+move:l1 l2 l3;elim:ll=>//=l4 ll hind l1 l2 l3 h123/#.
+qed.
+
+lemma prefixe_lt_size (l : 'a list) (ll : 'a list list) :
+    prefixe l (get_max_prefixe l ll) < size l =>
+    forall i, prefixe l (get_max_prefixe l ll) < i =>
+    ! take i l \in ll.
+proof.
+move:l;elim:ll=>//=l2 ll Hind l1;clear Hind;move:l1 l2;elim:ll=>//=.
++ progress.
+  rewrite-(cat_take_drop (prefixe l1 l2) (take i l1))
+    -{3}(cat_take_drop (prefixe l1 l2) l2)take_take/min H0/=.
+  rewrite prefixe_take. 
+  cut:drop (prefixe l1 l2) (take i l1) <> drop (prefixe l1 l2) l2;2:smt(catsI). 
+  rewrite (prefixe_take_geq_prefixe l1 l2 i) 1:/#.  
+  cut:=drop_prefixe_neq (take i l1) l2.
+  cut/#:drop (prefixe (take i l1) l2) (take i l1) <> [].
+  cut:0 < size (drop (prefixe (take i l1) l2) (take i l1));2:smt(size_eq0).
+  rewrite size_drop 1:prefixe_ge0 size_take;1:smt(prefixe_ge0).
+  by rewrite-prefixe_take_geq_prefixe /#.
+
+move=>l3 ll hind l1 l2.
+case(prefixe l1 l2 < prefixe l1 l3)=>//=h;progress.
++ rewrite!negb_or/=. 
+  cut:=hind l1 l3 H i H0;rewrite negb_or=>[][->->]/=.
+  cut:=hind l1 l2 _ i _;smt(prefixe_prefixe_prefixe).
+smt(prefixe_prefixe_prefixe).
+qed.
+
+lemma asfadst queries prefixes (bs : block list) :
+    prefixe_inv queries prefixes =>
+    elems (dom queries ) <> [] =>
+    all_prefixes prefixes =>
+    (forall j, 0 <= j <= size bs => take j bs \in dom prefixes) => 
+    take (prefixe bs (get_max_prefixe bs (elems (dom queries))) + 1) bs = bs.
+proof.
+progress. 
+cut h:=prefixe_inv_leq bs (size bs) prefixes queries _ _ _ _ _;rewrite//=.
++ exact size_ge0.
++ rewrite H2//=;exact size_ge0.
+cut->/=:prefixe bs (get_max_prefixe bs (elems (dom queries))) = size bs by smt(prefixe_sizel).
+rewrite take_oversize/#.
+qed.
+
+
+lemma prefixe_exchange_prefixe_inv (ll1 ll2 : 'a list list) (l : 'a list) :
+    (forall l2, l2 \in ll1 => l2 \in ll2) =>
+    (forall (l2 : 'a list), l2 \in ll1 => forall i, take i l2 \in ll2) =>
+    (forall l2, l2 \in ll2 => exists l3, l2 ++ l3 \in ll1) =>
+    prefixe l (get_max_prefixe l ll1) = prefixe l (get_max_prefixe l ll2).
+proof.
+case(ll1 = [])=>//=[->/#|]//=ll1_nil.
+move=>incl all_prefix incl2 ;cut ll2_nil:ll2 <> [] by rewrite/#.
+cut:=get_max_prefixe_max l ll2 (get_max_prefixe l ll1) _.
++ by rewrite incl mem_get_max_prefixe ll1_nil.
+cut mem_ll2:=mem_get_max_prefixe l ll2 ll2_nil.
+cut[]l3 mem_ll1:=incl2 _ mem_ll2.
+cut:=get_max_prefixe_max l ll1 _ mem_ll1.
+smt(prefixeC prefixe_leq_prefixe_cat).
+qed.
+
+lemma prefixe_inv_nil queries prefixes :
+    prefixe_inv queries prefixes =>
+    elems (dom queries) = [] => dom prefixes <= fset1 [].
+proof.
+move=>[h1 [h2 h3]] h4 x h5;rewrite in_fset1.
+cut:=h3 x (size x).
+rewrite take_size h5/=;apply absurd=>//=h6.
+rewrite h6/=negb_exists/=;smt(memE).
+qed.
+
+
+lemma aux_prefixe_exchange queries prefixes (l : block list) :
+    prefixe_inv queries prefixes => all_prefixes prefixes =>
+    elems (dom queries) <>  [] =>
+    prefixe l (get_max_prefixe l (elems (dom queries))) = 
+    prefixe l (get_max_prefixe l (elems (dom prefixes))).
+proof.
+move=>[h1[h2 h3]] h5 h4;apply prefixe_exchange_prefixe_inv.
++ smt(memE take_size).
++ smt(memE).
+move=>l2;rewrite-memE=> mem_l2.
+case(l2=[])=>//=hl2;1:rewrite hl2/=. 
++ move:h4;apply absurd=>//=;rewrite negb_exists/=/#.
+smt(memE take_size).
+qed.
+
+lemma prefixe_exchange queries prefixes (l : block list) :
+    prefixe_inv queries prefixes => all_prefixes prefixes =>
+    prefixe l (get_max_prefixe l (elems (dom queries))) = 
+    prefixe l (get_max_prefixe l (elems (dom prefixes))).
+proof.
+move=>[h1[h2 h3]] h5.
+case(elems (dom queries) = [])=>//=h4;2:smt(aux_prefixe_exchange).
+cut h6:=prefixe_inv_nil queries prefixes _ h4;1:rewrite/#.
+rewrite h4/=. search FSet.(<=).
+case(elems (dom prefixes) = [])=>//=[->//=|]h7.
+cut h8:elems (dom prefixes) = [[]].
++ cut [hh1 hh2]:[] \in dom prefixes /\ forall x, x \in elems (dom prefixes) => x = [] by smt(memE).
+  cut h9:=subset_leq_fcard _ _ h6.
+  apply (eq_from_nth witness)=>//=.
+  + rewrite-cardE-(fcard1 [<:block>]);move:h9;rewrite!fcard1!cardE=>h9. 
+    cut/#:0 < size (elems (dom prefixes));smt(size_eq0 size_ge0 fcard1).
+  move:h9;rewrite!fcard1!cardE=>h9 i [hi0 hi1]. 
+  cut->/=:i = 0 by rewrite/#.
+  by apply hh2;rewrite mem_nth/#.
+by rewrite h8=>//=.  
+qed.
+
+
+(* lemma prefixe_inv_prefixe queries prefixes l : *)
+(*     prefixe_inv queries prefixes => *)
+(*     all_prefixes prefixes => *)
+(*     (elems (dom queries) = [] => elems (dom prefixes) = [[]]) => *)
+(*     prefixe l (get_max_prefixe l (elems (dom queries))) =  *)
+(*     prefixe l (get_max_prefixe l (elems (dom prefixes))). *)
+(* proof. *)
+(* move=>[? h_prefixe_inv] h_all_prefixes. *)
+(* case(elems (dom queries) = [])=>//=h_nil. *)
+(* + by rewrite h_nil//==>->/=. *)
+(* cut h_mem_queries:=mem_get_max_prefixe l (elems (dom queries)) h_nil. *)
+(* cut h_leq :=all_take_in l (prefixe l (get_max_prefixe l (elems (dom queries)))) _ _ h_all_prefixes _. *)
+(* + smt(prefixe_ge0 prefixe_sizel). *)
+(* + by rewrite prefixe_take h_prefixe_inv memE h_mem_queries. *)
+(* cut:=all_take_in l (prefixe l (get_max_prefixe l (elems (dom prefixes)))) _ _ h_all_prefixes _. *)
+(* + smt(prefixe_ge0 prefixe_sizel). *)
+(* +  *)
+(* rewrite prefixe_take. *)
+  
+(*   rewrite -take_size. *)
+
+(* print mem_get_max_prefixe. *)
+
+(* qed. *)
 
 pred invm (m mi : ('a * 'b, 'a * 'b) fmap) =
   forall x y, m.[x] = Some y <=> mi.[y] = Some x.
@@ -306,67 +758,73 @@ by rewrite/=-2!cats1 blocksponge_cat/=.
 qed.
 
 
-pred prefixe_inv (queries : (block list, block) fmap)
-               (m : (state, state) fmap) =
-  forall (bs : block list),
-    bs \in dom queries =>
-    forall i, 0 <= i < size bs =>
-      let bc  = (blocksponge (take i bs) m s0).`2 in
-      (bc.`1 +^ nth b0 bs i, bc.`2) \in dom m.
+(* lemma prefixe_inv_bs_fst_nil queries prefixes m : *)
+(*     prefixe_inv queries prefixes m => *)
+(*     forall l, l \in dom queries => *)
+(*     forall i, 0 <= i <= size l => *)
+(*     (blocksponge (take i l) m s0).`1 = []. *)
+(* proof. *)
+(* move=>[h2 [h3 Hinv]] l Hdom i [Hi0 Hisize];move:i Hi0 l Hisize Hdom;apply intind=>//=. *)
+(* + by move=>l;rewrite take0/=. *)
+(* move=>i Hi0 Hind l Hil Hldom. *)
+(* rewrite(take_nth b0)1:/#. *)
+(* rewrite blocksponge_rcons/=. *)
+(* cut->/=:=Hind l _ Hldom;1:rewrite/#. *)
+(* by cut/=->/=/#:=Hinv _ Hldom i. *)
+(* qed. *)
 
 
-
-lemma prefixe_inv_bs_fst_nil queries m :
-    prefixe_inv queries m =>
-    forall l, l \in dom queries =>
-    forall i, 0 <= i <= size l =>
-    (blocksponge (take i l) m s0).`1 = [].
-proof.
-move=>Hinv l Hdom i [Hi0 Hisize];move:i Hi0 l Hisize Hdom;apply intind=>//=.
-+ by move=>l;rewrite take0/=.
-move=>i Hi0 Hind l Hil Hldom.
-rewrite(take_nth b0)1:/#.
-rewrite blocksponge_rcons/=.
-cut->/=:=Hind l _ Hldom;1:rewrite/#.
-by cut/=->/=:=Hinv _ Hldom i _;1:rewrite/#.
-qed.
+(* lemma blocksponge_drop l m bc : *)
+(*     exists i, 0 <= i <= List.size l /\ (blocksponge l m bc).`1 = drop i l. *)
+(* proof. *)
+(* move:l bc=>l;elim:l=>//=;1:exists 0=>//=;progress. *)
+(* case((bc.`1 +^ x, bc.`2) \in dom m)=>//=h. *)
+(* + cut[i [[hi0 His] Hi]]:=H (oget m.[(bc.`1 +^ x, bc.`2)]). *)
+(*   exists(i+1)=>/#. *)
+(* cut[i [[hi0 His] Hi]]:=H (oget m.[(bc.`1 +^ x, bc.`2)]). *)
+(* exists 0=>/#. *)
+(* qed. *)
 
 
-lemma prefixe_inv_set queries m x y :
-    !x \in dom m =>
-    prefixe_inv queries m =>
-    prefixe_inv queries m.[x <- y].
-proof.
-move=>Hxdom Hpref bs/=Hbsdom i [Hi0 Hisize].
-cut->:blocksponge (take i bs) m.[x <- y] s0 = blocksponge (take i bs) m s0.
-+ move:i Hi0 bs Hisize Hbsdom;apply intind=>//=i;first by rewrite take0//=.
-  move=>Hi0 Hind bs Hsize Hbsdom.
-  rewrite (take_nth b0)1:/#.
-  rewrite 2!blocksponge_rcons/=.
-  cut->/=:=prefixe_inv_bs_fst_nil _ _ Hpref _ Hbsdom i _;1:rewrite/#.
-  cut/=->/=:=Hpref _ Hbsdom i _;1:rewrite/#.
-  cut->/=:=Hind bs _ Hbsdom;1:rewrite/#.
-  cut->/=:=prefixe_inv_bs_fst_nil _ _ Hpref _ Hbsdom i _;1:rewrite/#.
-  rewrite dom_set in_fsetU1.
-  cut/=->/=:=Hpref _ Hbsdom i _;1:rewrite/#.
-  rewrite getP.
-  cut/#:=Hpref _ Hbsdom i _;1:rewrite/#.
-rewrite dom_set in_fsetU1.
-cut/#:=Hpref _ Hbsdom i _;1:rewrite/#.
-qed.
+(* lemma prefixe_inv_set queries prefixes m x y : *)
+(*     !x \in dom m => *)
+(*     prefixe_inv queries prefixes m => *)
+(*     prefixe_inv queries prefixes m.[x <- y]. *)
+(* proof. *)
+(* move=>Hxdom Hpref;progress=>//=.  *)
+(* + rewrite/#. *)
+(* + rewrite/#. *)
+(* cut->:blocksponge (take i bs) m.[x <- y] s0 = blocksponge (take i bs) m s0. *)
+(* + move:i H2  bs H3 H1;apply intind=>//=i;first smt(take0). *)
+(*   move=>Hi0 Hind bs Hisize Hbsdom. *)
+(*   rewrite (take_nth b0)1:/#. *)
+(*   rewrite 2!blocksponge_rcons/=. *)
+(*   cut[?[? Hpre]]:=Hpref. *)
+(*   cut->/=:=prefixe_inv_bs_fst_nil _ _ _ Hpref _ Hbsdom i _;1:rewrite/#. *)
+(*   cut/=->/=:=Hpre _ Hbsdom i _;1:rewrite/#. *)
+(*   cut->/=:=Hind bs _ Hbsdom;1:rewrite/#. *)
+(*   cut->/=:=prefixe_inv_bs_fst_nil _ _ _ Hpref _ Hbsdom i _;1:rewrite/#. *)
+(*   rewrite dom_set in_fsetU1. *)
+(*   cut/=->/=:=Hpre _ Hbsdom i _;1:rewrite/#. *)
+(*   rewrite getP. *)
+(*   cut/#:=Hpre _ Hbsdom i _;1:rewrite/#. *)
+(* rewrite dom_set in_fsetU1. *)
+(* cut[?[? Hpre]]:=Hpref. *)
+(* cut/#:=Hpre _ H1 i _;1:rewrite/#. *)
+(* qed. *)
 
 
-lemma blocksponge_set_nil l m bc x y :
-    !x \in dom m =>
-    let bs1 = blocksponge l m bc in
-    let bs2 = blocksponge l m.[x <- y] bc in
-    bs1.`1 = [] =>
-    bs2 = ([], bs1.`2).
-proof.
-rewrite/==>hdom bs1.
-cut/=:=blocksponge_set l m bc x y.
-smt(size_ge0 size_eq0).
-qed.
+(* lemma blocksponge_set_nil l m bc x y : *)
+(*     !x \in dom m => *)
+(*     let bs1 = blocksponge l m bc in *)
+(*     let bs2 = blocksponge l m.[x <- y] bc in *)
+(*     bs1.`1 = [] => *)
+(*     bs2 = ([], bs1.`2). *)
+(* proof. *)
+(* rewrite/==>hdom bs1. *)
+(* cut/=:=blocksponge_set l m bc x y. *)
+(* smt(size_ge0 size_eq0). *)
+(* qed. *)
 
 (* lemma size_blocksponge queries m l : *)
 (*     prefixe_inv queries m => *)
@@ -388,13 +846,9 @@ export Prefixe.
 
 module C = {
   var c  : int
-  var m  : (state, state) fmap
-  var mi : (state, state) fmap
   var queries : (block list, block) fmap
-  proc init () = { 
+  proc init () = {
     c       <- 0;
-    m       <- map0;
-    mi      <- map0;
     queries <- map0;
   }
 }.
@@ -408,31 +862,15 @@ module PC (P:PRIMITIVE) = {
 
   proc f (x:state) = {  
     var y <- (b0,c0);
-    if (!x \in dom C.m) {
-      y        <@ P.f(x);
-      C.c      <- C.c + 1;
-      C.m.[x]  <- y;
-      if (! y \in dom C.mi) {
-        C.mi.[y] <- x;
-      }
-    } else {
-      y        <- oget C.m.[x];
-    }
+    y        <@ P.f(x);
+    C.c      <- C.c + 1;
     return y;
   }
 
   proc fi(x:state) = {
     var y <- (b0,c0);
-    if (!x \in dom C.mi) {
-      y        <@ P.fi(x);
-      C.c      <- C.c + 1;
-      C.mi.[x] <- y;
-      if (! y \in dom C.m) {
-        C.m.[y]  <- x;
-      }
-    } else {
-      y        <- oget C.mi.[x];
-    }
+    y        <@ P.fi(x);
+    C.c      <- C.c + 1;
     return y;
   } 
 
@@ -442,34 +880,18 @@ module DPRestr (P:DPRIMITIVE) = {
 
   proc f (x:state) = {  
     var y <- (b0,c0);
-    if (!x \in dom C.m) {
-      if (C.c + 1 <= max_size) {
-        y        <@ P.f(x);
-        C.c      <- C.c + 1;
-        C.m.[x]  <- y;
-        if (! y \in dom C.mi) {
-          C.mi.[y] <- x;
-        }
-      }
-    } else {
-      y          <- oget C.m.[x];
+    if (C.c + 1 <= max_size) {
+      y        <@ P.f(x);
+      C.c      <- C.c + 1;
     }
     return y;
   }
 
   proc fi(x:state) = {
     var y <- (b0,c0);
-    if (!x \in dom C.mi) {
-      if (C.c + 1 <= max_size) {
-        y        <@ P.fi(x);
-        C.c      <- C.c + 1;
-        C.mi.[x] <- y;
-        if (! y \in dom C.m) {
-          C.m.[y]  <- x;
-        }
-      }
-    } else {
-      y          <- oget C.mi.[x];
+    if (C.c + 1 <= max_size) {
+      y        <@ P.fi(x);
+      C.c      <- C.c + 1;
     }
     return y;
   } 
@@ -491,7 +913,9 @@ module PRestr (P:PRIMITIVE) = {
 
 module FC(F:FUNCTIONALITY) = {
 
-  proc init = F.init
+  proc init() = {
+    F.init();
+  }
 
   proc f (bs:block list) = {
     var b <- b0;
@@ -525,7 +949,10 @@ module DFRestr(F:DFUNCTIONALITY) = {
 
 module FRestr(F:FUNCTIONALITY) = {
 
-  proc init = F.init
+  proc init() = {
+    Redo.init();
+    F.init();
+  }
 
   proc f = DFRestr(F).f 
 
@@ -543,10 +970,10 @@ module DRestr(D:DISTINGUISHER, F:DFUNCTIONALITY, P:DPRIMITIVE) = {
 }.
 
 lemma rp_ll (P<:DPRIMITIVE{C}): islossless P.f => islossless DPRestr(P).f.
-proof. move=>Hll;proc;sp;if;auto;if;auto;call Hll;auto. qed.
+proof. move=>Hll;proc;sp;if;auto;call Hll;auto. qed.
 
 lemma rpi_ll (P<:DPRIMITIVE{C}): islossless P.fi => islossless DPRestr(P).fi.
-proof. move=>Hll;proc;sp;if;auto;if;auto;call Hll;auto. qed.
+proof. move=>Hll;proc;sp;if;auto;call Hll;auto. qed.
 
 lemma rf_ll (F<:DFUNCTIONALITY{C}): islossless F.f => islossless DFRestr(F).f.
 proof. move=>Hll;proc;sp;if;auto;if=>//;auto;call Hll;auto. qed.
@@ -575,8 +1002,9 @@ section RESTR.
     Pr[Indif(FRestr(F), PRestr(P), D).main()@ &m: res] =
     Pr[Indif(F,P,DRestr(D)).main()@ &m: res].
   proof.
-    byequiv=>//.
-    proc;inline *;wp;swap{1}1 2;sim;auto;call(:true);auto;call(:true);auto. 
+    byequiv=>//;auto.
+    proc;inline *;wp. 
+    swap{1}[1..2] 3;sim;auto;call(:true);auto. 
   qed.
 
 end section RESTR.
@@ -602,22 +1030,22 @@ section COUNT.
   proof.
     byequiv (_: ={glob D, glob P, glob CO} ==> C.c{1} <= max_size => ={res})=>//;
       2:by move=> ??H[]?/H<-.
-    symmetry;proc;inline *;wp;swap{2}1 2.
+    symmetry;proc;inline *;wp.
     call (_: max_size < C.c, ={glob P, glob CO, glob C}).
     + apply D_ll.
-    + proc; sp;if;auto;if{1};1:by auto;call(_:true);auto. 
-      by call{2} f_ll;auto=>/#. 
-    + by move=> ?_;proc;sp;if;auto;if;auto;call f_ll;auto.
-    + by move=> _;proc;sp;if;auto;call f_ll;auto=>/#.
-    + proc;sp;if;auto;if{1};1:by auto;call(_:true);auto.
+    + proc; sp;if{1};1:by auto;call(_:true);auto. 
+      by auto;call{2} f_ll;auto=>/#. 
+    + by move=> ?_;proc;sp;auto;if;auto;call f_ll;auto.
+    + by move=> _;proc;sp;auto;call f_ll;auto=>/#.
+    + proc;sp;auto;if{1};1:by auto;call(_:true);auto.
       by call{2} fi_ll;auto=>/#. 
-    + by move=> ?_;proc;sp;if;auto;if;auto;call fi_ll;auto.
-    + by move=> _;proc;sp;if;auto;call fi_ll;auto=>/#.
+    + by move=> ?_;proc;sp;auto;if;auto;call fi_ll;auto.
+    + by move=> _;proc;sp;auto;call fi_ll;auto=>/#.
     + proc;inline*;sp 1 1;if;auto;if{1};auto;1:by call(_: ={glob P});auto;sim.
       by call{2} CO_ll;auto=>/#.
     + by move=> ?_;proc;sp;if;auto;if;auto;call CO_ll;auto.
     + by move=> _;proc;sp;if;auto;call CO_ll;auto;smt(prefixe_sizel).
-    wp;call (_:true);call(_:true);auto=>/#.
+    auto;call (_:true);auto;call(:true);auto=>/#.
   qed.
 
 end section COUNT.
